ATC4.thy
@@ -271,11 +271,11 @@ qed
 fun append_io_B :: "('in, 'out, 'state) FSM \<Rightarrow> ('in * 'out) list \<Rightarrow> ('in, 'out) ATC set \<Rightarrow> ('in * 'out) list set" where
 "append_io_B M io \<Omega> = { io@res | res . res \<in> B M io \<Omega> }"
 
-fun is_reduction_on :: "('in, 'out, 'state) FSM \<Rightarrow> ('in, 'out, 'state) FSM \<Rightarrow> 'in list \<Rightarrow> ('in, 'out) ATC set \<Rightarrow> bool" where
+fun is_reduction_on :: "('in, 'out, 'state1) FSM \<Rightarrow> ('in, 'out, 'state2) FSM \<Rightarrow> 'in list \<Rightarrow> ('in, 'out) ATC set \<Rightarrow> bool" where
 "is_reduction_on M1 M2 iseq \<Omega> = (language_state_in M1 (initial M1) {iseq} \<subseteq> language_state_in M2 (initial M2) {iseq} 
   \<and> (\<forall> io \<in> language_state_in M1 (initial M1) {iseq} . append_io_B M1 io \<Omega> \<subseteq> append_io_B M2 io \<Omega>))"
 
-fun is_reduction_on_sets :: "('in, 'out, 'state) FSM \<Rightarrow> ('in, 'out, 'state) FSM \<Rightarrow> 'in list set \<Rightarrow> ('in, 'out) ATC set \<Rightarrow> bool" where
+fun is_reduction_on_sets :: "('in, 'out, 'state1) FSM \<Rightarrow> ('in, 'out, 'state2) FSM \<Rightarrow> 'in list set \<Rightarrow> ('in, 'out) ATC set \<Rightarrow> bool" where
 "is_reduction_on_sets M1 M2 TS \<Omega> = (\<forall> iseq \<in> TS . is_reduction_on M1 M2 iseq \<Omega>)"
 
 
